src/LibMap.v
@@ -1,12 +1,3 @@
-
-
-
-
-(** DISCLAIMER: file under construction *)
-
-
-
-
 (**************************************************************************
 * TLC: A library for Coq                                                  *
 * Finite maps                                                             *
@@ -19,14 +10,6 @@ Require Import LibTactics LibLogic LibReflect LibOption
 Require Export LibContainer.
 
 Local Open Scope set_scope.
-
-(* ---------------------------------------------------------------------- *)
-(** ** Notations to help the typechecker *)
-
-Notation "x \indom E" := (x \in (dom E : set _))
-  (at level 39) : container_scope.
-Notation "x \notindom E" := (x \notin ((dom E) : set _))
-  (at level 39) : container_scope.
 
 
 (* ********************************************************************** *)
@@ -74,7 +57,7 @@ Definition disjoint_impl M N :=
 Definition index_impl M k :=
   k \in (dom_impl M : set A).
 
-(* todo: incl_impl *)
+(* -- TODO: incl_impl *)
 
 End Operations.
 
@@ -84,7 +67,7 @@ Definition read_impl A `{Inhab B} (M:map A B) (k:A) :=
   | Some v => v
   end.
 
-Definition fold_impl A B C (m:monoid_def C) (f:A->B->C) (M:map A B) :=
+Definition fold_impl A B C (m:monoid_op C) (f:A->B->C) (M:map A B) :=
   LibContainer.fold m (fun p => let '(a,b) := p in f a b)
     (\set{ p | exists k x, p = (k, x) /\ binds_impl M k x }).
 
@@ -94,24 +77,34 @@ Definition fold_impl A B C (m:monoid_def C) (f:A->B->C) (M:map A B) :=
 
 Instance empty_inst : forall A B, BagEmpty (map A B).
   constructor. rapply (@empty_impl A B). Defined.
+
 Instance single_bind_inst : forall A B, BagSingleBind A B (map A B).
   constructor. rapply (@single_bind_impl A B). Defined.
+
 Instance binds_inst : forall A B, BagBinds A B (map A B).
   constructor. rapply (@binds_impl A B). Defined.
-Instance union_inst : forall A B, BagUnion (map A B). (* todo: bug pas si on enelve B *)
+
+Instance union_inst : forall A B, BagUnion (map A B).
   constructor. rapply (@union_impl A B). Defined.
+
 Instance remove_inst : forall A B, BagRemove (map A B) (set A).
   constructor. rapply (@remove_impl A B). Defined.
+
 Instance restrict_inst : forall A B, BagRestrict (map A B) (set A).
   constructor. rapply (@restrict_impl A B). Defined.
+
 Instance read_inst : forall A `{Inhab B}, BagRead A B (map A B).
   constructor. rapply (@read_impl A B H). Defined.
+
 Instance dom_inst : forall A B, BagDom (map A B) (set A).
   constructor. rapply (@dom_impl A B). Defined.
+
 Instance disjoint_inst : forall A B, BagDisjoint (map A B).
   constructor. rapply (@disjoint_impl A B). Defined.
+
 Instance index_inst : forall A B, BagIndex A (map A B).
   constructor. rapply (@index_impl A B). Defined.
+
 Instance fold_inst : forall A B C, BagFold C (A->B->C) (map A B).
   constructor. rapply (@fold_impl A B C). Defined.
 
@@ -123,14 +116,18 @@ Instance Inhab_map : forall A, Inhab (map A B).
 Proof using. intros. apply (Inhab_of_val (@empty_impl A B)). Qed.
 
 
-(* Check that update is derivable via bag_update_as_union_single
-    Instance update_inst : forall A B, BagUpdate A B (map A B).
-    Proof. typeclass. Qed. *)
+(* Note: we may check that [update] is derivable via [bag_update_as_union_single]
+      Instance update_inst : forall A B, BagUpdate A B (map A B).
+      Proof. typeclass. Qed. 
+*)
+
 
 (* ********************************************************************** *)
 (* Extra definitons *)
 
-Definition finite A B (M:map A B) :=  (* TODO: will become a typeclass *)
+(*-- LATER: make [finite] a typeclass *)
+
+Definition finite A B (M:map A B) :=
   finite (dom M).
 
 
@@ -143,16 +140,16 @@ Transparent map empty_inst single_bind_inst binds_inst
  union_inst restrict_inst remove_inst read_inst
  dom_inst disjoint_inst index_inst fold_inst.
 
-Lemma binds_def : forall A `{Inhab B} (M:map A B) x v,
+Lemma binds_eq_indom_read : forall A `{Inhab B} (M:map A B) x v,
   binds M x v = (x \indom M /\ M[x] = v).
 Proof using.
   intros. simpl. unfold dom_impl, read_impl, binds_impl.
-  extens. set_norm. iff R (N&R).
+  extens. rew_set. iff R (N&R).
     rewrite R. split~. congruence.
     destruct (M x). subst~. false.
 Qed.
 
-Lemma dom_def_binds : forall A B (M:map A B),
+Lemma dom_eq_set_of_binds : forall A B (M:map A B),
   dom M = \set{ k | exists v, binds M k v }.
 Proof using.
   intros. simpl. unfold dom_impl, binds_impl.
@@ -161,36 +158,33 @@ Proof using.
     destruct R. congruence.
 Qed.
 
-Lemma index_def : forall A B (M:map A B) k,
-  index M k = (k \in (dom M : set A)).
+Lemma index_eq_indom : forall A B (M:map A B) k,
+  index M k = (k \indom M).
 Proof using. auto. Qed.
 
-Lemma disjoint_def : forall A B (M N:map A B),
+Lemma disjoint_eq_disjoint_dom : forall A B (M N:map A B),
   disjoint M N = disjoint (dom M) (dom N).
 Proof using. auto. Qed.
 
-Lemma fold_def_binds : forall A B C (m:monoid_def C) (f:A->B->C) (M:map A B),
+Lemma fold_eq_fold_pairs : forall A B C (m:monoid_op C) (f:A->B->C) (M:map A B),
   fold m f M = LibContainer.fold m (fun p => let '(a,b) := p in f a b)
     (\set{ p | exists k x, p = (k, x) /\ binds_impl M k x }).
 Proof using. auto. Qed.
 
-Lemma update_def_union : forall A B (M:map A B) k x,
+Lemma update_eq_union_single : forall A B (M:map A B) k x,
   M[k:=x] = M \u (k \:= x).
 Proof using. auto. Qed.
 
 (* only for internal use *)
-Lemma update_def_if : forall A B (M:map A B) k x,
+Lemma update_impl_eq : forall A B (M:map A B) k x,
   M[k:=x] = (fun k' => If k = k' then Some x else M k').
 Proof using.
-  intros. rewrite update_def_union.
+  intros. rewrite update_eq_union_single.
   simpl. unfold single_bind_impl, union_impl.
   apply fun_ext_1. intros k'. case_if~.
 Qed.
 
 End Reformulation.
-
-
-(* Hint Resolve index_of_indom. *)
 
 
 (* ********************************************************************** *)
@@ -214,8 +208,9 @@ Hint Extern 1 (None <> Some _) => congruence.
 (** index *)
 
 Lemma index_of_indom : forall A B (M:map A B) k,
-  k \indom M -> index M k.
-Proof using. intros. rewrite~ index_def. Qed.
+  k \indom M -> 
+  index M k.
+Proof using. intros. rewrite~ index_eq_indom. Qed.
 
 
 (* ---------------------------------------------------------------------- *)
@@ -234,20 +229,21 @@ Lemma dom_single : forall A B (k:A) (x:B),
 Proof using.
   intros. simpl. unfold binds_impl, single_bind_impl, dom_impl.
   apply set_ext. intros y. rewrite in_set_st_eq. iff R; case_if~.
+  rewrite in_single_eq. auto.
 Qed.
 
 Lemma dom_union : forall A B (M N : map A B),
   dom (M \u N) = dom M \u dom N.
 Proof using.
   intros. simpl. unfold dom_impl, union_impl.
-  set_norm. intros x. set_norm. iff R; destruct* (N x).
+  rew_set. intros x. rew_set. iff R; destruct* (N x).
 Qed.
 
 
 (* ---------------------------------------------------------------------- *)
 (** indom *)
 
-Lemma in_dom_empty : forall A B x,
+Lemma indom_empty_inv : forall A B x,
   x \indom (\{} : map A B) ->
   False.
 Proof using.
@@ -258,177 +254,213 @@ Qed.
 (* ---------------------------------------------------------------------- *)
 (** prove empty *)
 
-Lemma no_binds_empty : forall (A B : Type) (M : map A B),
-  (forall x k, ~ binds M x k) -> M = \{}.
+Lemma eq_empty_of_not_binds : forall (A B : Type) (M : map A B),
+  (forall x k, ~ binds M x k) -> 
+  M = \{}.
 Proof using.
   intros A B M. simpl. unfold empty_impl, binds_impl.
   intros H. apply fun_ext_1. intros x. cases (M x); auto_false*.
 Qed.
 
 Lemma dom_empty_inv : forall A B (M : map A B),
-  dom M = \{} -> M = \{}.
+  dom M = \{} -> 
+  M = \{}.
 Proof using.
   introv H. simpls. unfold dom_impl, empty_impl in *.
-  apply fun_ext_1. (* todo: "extens" should work *) intros k.
-  absurds as G.
-  lets R: @is_empty_inv k H. typeclass. false R. rewrite~ in_set_st_eq.
-Qed. (* todo: simplify proof *)
+  extens ;=> k. absurds ;=> G.
+  lets R: @is_empty_inv k H. typeclass.
+  false R. rewrite~ in_set_st_eq.
+Qed.
 
 
 (* ---------------------------------------------------------------------- *)
 (** update *)
 
-
-(* TODO: how to choose between index and indom to state side conditions? *)
-
 (* dom *)
 
 Lemma dom_update : forall A B i v (M:map A B),
-  dom (M[i:=v]) = dom M \u \{i}.
+  dom (M[i:=v]) = (dom M \u \{i}).
 Proof using.
-  intros. rewrite update_def_if.
+  intros. rewrite update_impl_eq.
   simpl. unfold dom_impl, union_impl, binds_impl in *.
   apply in_extens.  (* "extens" should work directly *)
-  intros x. set_norm. iff R.
+  intros x. rew_set. iff R.
     case_if~.
     case_if~. destruct~ R.
 Qed.
 
-Lemma dom_update_index : forall A i `{Inhab B} v (M:map A B), (* needed? *)
+Open Scope container_scope.
+
+Lemma dom_update_at_indom : forall A i `{IB:Inhab B} v (M:map A B),
+  i \indom M ->
+  dom (M[i:=v]) = dom M.
+Proof using.
+  introv IB H. rewrite dom_update.
+  set_prove_setup true. tests*: (x = i). 
+  (* --LATER: improve "set_prove" ? *)
+Qed.
+
+Arguments dom_update_at_indom [A] i [B] {IB}.
+
+(* -- LATER: Is it needed to have the form with [index] as hyp? *)
+Lemma dom_update_at_index : forall A i `{IB:Inhab B} v (M:map A B),
   index M i ->
   dom (M[i:=v]) = dom M.
 Proof using.
-  introv IB H. rewrite index_def in H. rewrite dom_update.
-  set_prove_setup true. tests*: (x = i). (* todo: improve "set_prove" ? *)
+  introv IB H. rewrite index_eq_indom in H. rewrite dom_update.
+  set_prove_setup true. tests*: (x = i). 
 Qed.
 
-Implicit Arguments dom_update_index [A B [H]].
-
-Lemma dom_update_index' : (* TODO: needed? *)
-  forall A `{Inhab B} (M M' : map A B) (D : set A) x v,
-  M' = M[x:=v] ->
-  D = dom M ->
-  x \in D ->
-  D = dom M'.
-Proof using. intros. subst. rewrite~ dom_update_index. Qed.
+Arguments dom_update_at_index [A] i [B] {IB}.
 
 (* indom *)
 
-Lemma indom_update : forall A `{Inhab B} (m:map A B) (i j:A) (v:B),
+Lemma indom_update_eq : forall A `{Inhab B} (m:map A B) (i j:A) (v:B),
   j \indom (m[i:=v]) = (j = i \/ j \indom m).
-Proof using. intros. rewrite dom_update. set_norm. extens*. Qed.
+Proof using. intros. rewrite dom_update. rew_set. extens*. Qed.
 
 Lemma indom_update_inv : forall A `{Inhab B} (m:map A B) (i j:A) (v:B),
-  j \indom (m[i:=v]) -> (j = i \/ j \indom m).
-Proof using. introv IB H. rewrite~ indom_update in H. Qed.
+  j \indom (m[i:=v]) -> 
+  (j = i \/ j \indom m).
+Proof using. introv IB H. rewrite~ indom_update_eq in H. Qed.
 
-Lemma indom_update_already_inv : forall A `{Inhab B} (m:map A B) (i j:A) (v:B),
-  j \indom (m[i:=v]) -> i \indom m -> j \indom m.
-Proof using. introv IB H F. rewrite~ indom_update in H. destruct~ H. subst~. Qed.
+Lemma indom_of_indom_update_at_indom : forall A `{Inhab B} (m:map A B) (i j:A) (v:B),
+  j \indom (m[i:=v]) -> 
+  i \indom m -> 
+  j \indom m.
+Proof using. introv IB H F. rewrite~ indom_update_eq in H. destruct~ H. subst~. Qed.
 
-Lemma indom_update_already : forall A `{Inhab B} (m:map A B) (i j:A) (v:B),
-  j \indom m -> j \indom (m[i:=v]).
-Proof using. intros. rewrite~ indom_update. Qed.
+Lemma indom_update_of_indom : forall A `{Inhab B} (m:map A B) (i j:A) (v:B),
+  j \indom m -> 
+  j \indom (m[i:=v]).
+Proof using. intros. rewrite~ indom_update_eq. Qed.
 
-Lemma indom_update_self : forall A `{Inhab B} (m:map A B) (i:A) (v:B),
+Lemma indom_update_same : forall A `{Inhab B} (m:map A B) (i:A) (v:B),
   i \indom (m[i:=v]).
-Proof using. intros. rewrite~ indom_update. Qed.
+Proof using. intros. rewrite~ indom_update_eq. Qed.
 
-Hint Resolve indom_update_self. (* TODO: move *)
+Hint Resolve indom_update_same. (* TODO: move *)
 
 (* update *)
 
-Lemma update_read_if : forall A `{Inhab B} (m:map A B) (i j:A) (v:B),
-  (m[i:=v])[j] = If i = j then v else m[j].
+Lemma read_update : forall A `{Inhab B} (m:map A B) (i j:A) (v:B),
+  (m[i:=v])[j] = (If i = j then v else m[j]).
 Proof using.
- intros. rewrite update_def_if. simpl. unfold read_impl. case_if~.
+ intros. rewrite update_impl_eq. simpl. unfold read_impl. case_if~.
 Qed.
 
-Lemma update_read_eq : forall A `{Inhab B} (m:map A B) (i:A) (v:B),
+Lemma read_update_same : forall A `{Inhab B} (m:map A B) (i:A) (v:B),
   (m[i:=v])[i] = v.
-Proof using. intros. rewrite update_read_if. case_if~. Qed.
+Proof using. intros. rewrite read_update. case_if~. Qed.
 
-Lemma update_read_neq : forall A `{Inhab B} (m:map A B) (i j:A) (v:B),
-  i<>j -> (m[i:=v])[j] = m[j].
-Proof using. intros. rewrite update_read_if. case_if~. Qed.
+Lemma read_update_neq : forall A `{Inhab B} (m:map A B) (i j:A) (v:B),
+  i <> j -> 
+  (m[i:=v])[j] = m[j].
+Proof using. intros. rewrite read_update. case_if~. Qed.
 
-Lemma update_update_eq : forall A i `{Inhab B} v v' (M:map A B),
+Lemma update_update : forall A i `{Inhab B} v v' (M:map A B),
   M[i:=v][i:=v'] = M[i:=v'].
 Proof using.
   intros. applys fun_ext_1.
-  intros k. do 3 rewrite update_def_if. case_if~.
+  intros k. do 3 rewrite update_impl_eq. case_if~.
 Qed.
 
 
 (* ---------------------------------------------------------------------- *)
 (** binds *)
 
-(* LATER: {Inhab B} could probably be removed below in many places *)
+(* ---TODO: {Inhab B} could probably be removed below in many places,
+            because [binds M i v] with [M:map A B] entails {Inhab B}. *)
 
-Lemma binds_prove : forall A `{Inhab B} (M:map A B) x v,
-  x \indom M -> M[x] = v -> binds M x v.
+Lemma binds_inj : forall A i `{Inhab B} v1 v2 (M:map A B),
+  binds M i v1 -> 
+  binds M i v2 -> 
+  v1 = v2.
 Proof using.
-  intros. rewrite~ (@binds_def A B H). (* why need explicit args? *)
+  introv IB H1 H2.
+  rewrite (@binds_eq_indom_read A B IB) in *.
+  destruct H1; destruct H2. congruence. (* todo: cleanup *)
 Qed.
 
-Lemma binds_dom : forall A `{Inhab B} (M:map A B) x v,
-  binds M x v -> x \indom M.
-Proof using. introv IB K. rewrite* (@binds_def A B IB) in K. Qed.
+Lemma binds_of_indom_read : forall A `{Inhab B} (M:map A B) x v,
+  x \indom M -> 
+  M[x] = v -> 
+  binds M x v.
+Proof using.
+  intros. rewrite~ (@binds_eq_indom_read A B H). (* why need explicit args? *)
+Qed.
 
-Lemma binds_index : forall A i `{Inhab B} v (M:map A B),
-  binds M i v -> index M i.
-Proof using. introv IB K. rewrite* (@binds_def A B IB) in K. Qed.
+Lemma indom_of_binds : forall A `{Inhab B} (M:map A B) x v,
+  binds M x v -> 
+  x \indom M.
+Proof using. introv IB K. rewrite* (@binds_eq_indom_read A B IB) in K. Qed.
 
-Lemma binds_read : forall A `{Inhab B} (M:map A B) x v,
-  binds M x v -> M[x] = v.
-Proof using. introv K. rewrite* (@binds_def A B H) in K. Qed.
+Lemma index_of_binds : forall A i `{Inhab B} v (M:map A B),
+  binds M i v -> 
+  index M i.
+Proof using. introv IB K. rewrite* (@binds_eq_indom_read A B IB) in K. Qed.
+
+Lemma read_of_binds : forall A `{Inhab B} (M:map A B) x v,
+  binds M x v -> 
+  M[x] = v.
+Proof using. introv K. rewrite* (@binds_eq_indom_read A B H) in K. Qed.
 
 Lemma binds_update_neq : forall A B i j v w (M:map A B),
-  i <> j -> binds M i v -> binds (M[j:=w]) i v.
+  i <> j -> 
+  binds M i v -> 
+  binds (M[j:=w]) i v.
 Proof using.
   introv N K. asserts IB: (Inhab B). constructor. exists* v.
-  rewrite (@binds_def A B IB) in *.
-  rewrite~ indom_update. rewrite* update_read_neq.
+  rewrite (@binds_eq_indom_read A B IB) in *.
+  rewrite~ indom_update_eq. rewrite* read_update_neq.
 Qed. (* later: cleanup proof *)
 
-Lemma binds_update_neq' : forall A i j `{Inhab B} v w (M:map A B), (* todo: needed? *)
-  i <> j -> binds M i v -> binds (M[j:=w]) i v.
-Proof using. intros. applys* binds_update_neq. Qed.
-
-Lemma binds_update_eq : forall A B i v (M:map A B),
+Lemma binds_update_same : forall A B i v (M:map A B),
   binds (M[i:=v]) i v.
 Proof using.
   intros.
   asserts IB: (Inhab B). constructor. exists* v.
-  rewrite (@binds_def A B IB) in *.
-  rewrite~ indom_update. rewrite* update_read_eq.
+  rewrite (@binds_eq_indom_read A B IB) in *.
+  rewrite~ indom_update_eq. rewrite* read_update_same.
 Qed.
 
-Lemma binds_update_eq_inv : forall A B i v w (M:map A B),
-  binds (M[i:=w]) i v -> v = w.
+Lemma binds_update_same_inv : forall A B i v w (M:map A B),
+  binds (M[i:=w]) i v -> 
+  v = w.
 Proof using.
   introv H.
   asserts IB: (Inhab B). constructor. exists* v.
-  rewrite (@binds_def A B IB) in *.
-  rewrite~ indom_update in H. rewrite* update_read_eq in H.
+  rewrite (@binds_eq_indom_read A B IB) in *.
+  rewrite~ indom_update_eq in H. rewrite* read_update_same in H.
 Qed.
 
 Lemma binds_update_neq_inv : forall A B i j v w (M:map A B),
-  binds (M[j:=w]) i v -> i <> j -> binds M i v.
+  binds (M[j:=w]) i v -> 
+  i <> j -> 
+  binds M i v.
 Proof using.
   introv H N.
   asserts IB: (Inhab B). constructor. exists* v.
-  rewrite (@binds_def A B IB) in *.
-  rewrite~ indom_update in H. rewrite* update_read_neq in H.
+  rewrite (@binds_eq_indom_read A B IB) in *.
+  rewrite~ indom_update_eq in H. rewrite* read_update_neq in H.
 Qed.
 
-Lemma binds_inj : forall A i `{Inhab B} v1 v2 (M:map A B),
-  binds M i v1 -> binds M i v2 -> v1 = v2.
+Lemma binds_update_eq : forall A B i j v w (M:map A B),
+  binds (M[j:=w]) i v = (If i = j then v = w else binds M i v).
 Proof using.
-  introv IB H1 H2.
-  rewrite (@binds_def A B IB) in *.
-  destruct H1; destruct H2. congruence. (* todo: cleanup *)
+  intros. applys prop_ext. iff H.
+  { case_if.
+    { subst. applys* binds_update_same_inv. }
+    { applys* binds_update_neq_inv. } }
+  { case_if.
+    { subst. applys* binds_update_same. }
+    { applys* binds_update_neq. } }
 Qed.
+
+Lemma binds_update_inv : forall A B i j v w (M:map A B),
+  binds (M[j:=w]) i v ->
+  (If i = j then v = w else binds M i v).
+Proof using. introv H. rewrite~ binds_update_eq in H. Qed.
 
 
 (* ---------------------------------------------------------------------- *)
@@ -441,7 +473,7 @@ Lemma union_read_l : forall A `{Inhab B} (m1 m2:map A B) (i:A),
 Proof.
   introv M D. rewrite set_disjoint_eq in D.
   simpl. unfold read_impl, union_impl. cases (m2 i).
-  { false D M. applys~ binds_dom. simpl. unfolds* binds_impl. }
+  { false D M. applys~ indom_of_binds. simpl. unfolds* binds_impl. }
     (* LATER: simplify line above *)
   { cases~ (m1 i). }
 Qed.
@@ -455,52 +487,9 @@ Proof.
   simpl. unfold read_impl, union_impl. cases (m2 i).
   { auto. } 
   { cases (m1 i) as C.
-    { false D M. applys~ binds_dom. simpl. unfolds* binds_impl. }
+    { false D M. applys~ indom_of_binds. simpl. unfolds* binds_impl. }
     (* LATER: simplify line above *)
     { auto. } }
-Qed.
-
-(* ---------------------------------------------------------------------- *)
-
-(* LATER: cleanup the three lemmas below *)
-
-(* FALSE
-Lemma binds_update_neq_inv' : forall A B i j v w (M:map A B),
-  binds (M[j:=w]) i v -> j \notindom M -> binds M i v.
-
-Lemma binds_update_neq_eq : forall A `{Inhab B} i j v w (M:map A B),
-  j \notindom M ->
-  (binds M i v = binds (M[j:=w]) i v).
-Proof using.
-  split; intros.
-  { eapply binds_update_neq; [ | eauto ].
-    assert (i \indom M). { eapply binds_index; eauto. }
-    intro. subst. unfold notin in *. tauto. }
-  { eauto using binds_update_neq_inv'. }
-Qed.
-
-*)
-
-Lemma binds_update_analysis : forall A B i j v w (M:map A B),
-  binds (M[j:=w]) i v ->
-  i <> j /\ binds M i v \/
-  i = j /\ v = w.
-Proof using.
-  intros. tests: (i = j).
-  right. forwards*: binds_update_eq_inv H.
-  left. forwards*: binds_update_neq_inv H.
-Qed.
-
-Lemma binds_update_indom_eq :
-  forall A B (M : map A B) a1 a2 b1 b2,
-  binds (M[a1:=b1]) a2 b2 =
-  (    (a2 <> a1 /\ binds M a2 b2) 
-    \/ (a2 = a1 /\ b2 = b1)).
-Proof using.
-  split. introv [ [ ? ? ] | [ ? ? ] ].
-  { eauto using binds_update_neq. }
-  { subst. eapply binds_update_eq. }
-  { eauto using binds_update_analysis. }
 Qed.
 
 
@@ -508,11 +497,11 @@ Qed.
 (** remove *)
 
 Lemma dom_remove : forall A B (M:map A B) E,
-  dom (M\-E) = dom M \- E.
+  dom (M\-E) = (dom M \- E).
 Proof using.
   intros. simpl. unfold remove_impl, dom_impl in *.
   apply in_extens.  (* "extens" should work directly *)
-  intros x. set_norm. iff R (R1&R2); case_if~.
+  intros x. rew_set. iff R (R1&R2); case_if~.
 Qed.
 
 
@@ -524,35 +513,37 @@ Lemma dom_remove_one : forall A B i (M:map A B),
 Proof using. intros. applys~ dom_remove. Qed. (* TODO: needed ? *)
 
 Lemma index_remove_one_in : forall A B i j (M:map A B),
-  index M j -> i <> j -> index (M\--i) j.
+  index M j -> 
+  i <> j -> 
+  index (M\--i) j.
 Proof using.
-  introv R N. rewrite index_def in *. rewrite dom_remove_one.
-  set_norm. auto. (* todo: "set_norm*" *)
+  introv R N. rewrite index_eq_indom in *. rewrite dom_remove_one.
+  rew_set. auto. (* todo: "rew_set*" *)
 Qed.
 
-Implicit Arguments index_remove_one_in [A B].
+Arguments index_remove_one_in [A] [B].
 
-Lemma update_remove_one_eq : forall A `{Inhab B} (m:map A B) (i:A) (v:B),
+Lemma remove_one_update : forall A `{Inhab B} (m:map A B) (i:A) (v:B),
   (m[i:=v] \- \{i}) = (m \- \{i}).
 Proof using.
   intros. applys fun_ext_1.
-  intros k. rewrite update_def_if.
+  intros k. rewrite update_impl_eq.
   simpl. unfold remove_impl. do 2 case_if~.
 Qed.
 
-Lemma remove_one_read_neq : forall A `{Inhab B} (M:map A B) i j,
+Lemma read_remove_one_neq : forall A `{Inhab B} (M:map A B) i j,
   i <> j ->
   (M\--i)[j] = M[j].
 Proof using.
   introv N. simpl. unfold remove_impl, read_impl. case_if~.
 Qed.
 
-Lemma remove_one_update_neq : forall A B (M:map A B) i j v,
+Lemma update_remove_one_neq : forall A B (M:map A B) i j v,
   i <> j ->
   (M\--i)[j:=v] = (M[j:=v] \--i).
 Proof using.
   introv N. applys fun_ext_1.
-  intros k. do 2 rewrite update_def_if.
+  intros k. do 2 rewrite update_impl_eq.
   simpl. unfold remove_impl. do 2 case_if~.
 Qed.
 
@@ -566,14 +557,14 @@ Lemma restrict_single : forall A (x:A) `{Inhab B} (M:map A B),
 Proof using.
   introv N. applys fun_ext_1.
   intros k. simpls. unfolds dom_impl, restrict_impl, single_bind_impl, read_impl.
-  set_norm. do 2 case_if~. destruct (M x); auto_false.
+  rew_set in *. do 2 case_if~. subst. destruct (M x); auto_false.
 Qed.
 
 
 (* ---------------------------------------------------------------------- *)
 (** structural decomposition *)
 
-Lemma split_restrict_remove : forall A (E:set A) B (M:map A B),
+Lemma eq_union_restrict_remove : forall A (E:set A) B (M:map A B),
   M = (M \- E) \u (M \| E).
 Proof using.
   intros. applys fun_ext_1.
@@ -581,62 +572,47 @@ Proof using.
   case_if~. destruct~ (M k).
 Qed.
 
-Lemma split_restrict_remove_single : forall A (x:A) B `{Inhab B} (M:map A B),
+Lemma eq_union_restrict_remove_one : forall A (x:A) B `{Inhab B} (M:map A B),
   x \indom M ->
   M = (M \- \{x}) \u (x \:= (M[x])).
 Proof using.
-  intros. rewrite~ <- restrict_single. apply split_restrict_remove.
+  intros. rewrite~ <- restrict_single. apply eq_union_restrict_remove.
 Qed.
 
-(* ---------------------------------------------------------------------- *)
-(** fold, equivalent definition *)
-
-(* TODO
-Lemma fold_def_dom : forall A `{Inhab B} C (m:monoid_def C) (f:A->B->C) (M:map A B),
-  fold m f M = LibContainer.fold m (fun k => f k (M[k])) (dom M).
-Proof using. (* LATER *) Qed.
-  - E = dom M
-  - repr L E
-  - fold f (map i E) = fold (fun x => f (i x)) E
-  - i = fun x => (x, M[x])
-  - injective i -> repr E L -> repr (LibSet.map i E) (LibList.map i L)
-  - injective i -> No_duplicates L -> No_dupliactes (map i L)
-  - repr E L -> repr E L' -> fold f E = fold f L'
-
-*)
 
 (* ---------------------------------------------------------------------- *)
 (** fold *)
 
-Lemma fold_empty : forall A B C (m:monoid_def C) (f:A->B->C),
+Lemma fold_empty : forall A B C (m:monoid_op C) (f:A->B->C),
   fold m f (\{}:map A B) = monoid_neutral m.
 Proof using.
-  intros. rewrite fold_def_binds.
+  intros. rewrite fold_eq_fold_pairs.
   match goal with |- context [ set_st ?X] =>
     cuts_rewrite (set_st X = \{}) end.
   rewrite~ fold_empty.
-  set_norm. intros [k x]. set_norm. iff (?&?&M&N) ?; tryfalse.
+  rew_set. intros [k x]. rew_set. iff (?&?&M&N) ?; tryfalse.
 Qed.
 
-Lemma fold_single : forall A B C (m:monoid_def C) (f:A->B->C) (k:A) (x:B),
+Lemma fold_single : forall A B C (m:monoid_op C) (f:A->B->C) (k:A) (x:B),
   Monoid m ->
   fold m f (k\:=x) = f k x.
 Proof using.
-  intros. rewrite fold_def_binds.
+  intros. rewrite fold_eq_fold_pairs.
   match goal with |- context [ set_st ?X] =>
     cuts_rewrite (set_st X = \{(k,x)}) end.
   rewrite~ fold_single.
-  set_norm. intros [k' x']. set_norm. iff (?&?&E&R) M.
+  rew_set. intros [k' x']. rew_set. iff (?&?&E&R) M.
     inverts E. hnf in R. simpls. unfolds single_bind_impl.
-     case_if~. inverts~ R.
+     case_if~. inverts~ R. subst~.
     inverts M. unfolds binds_impl. simpls. unfolds single_bind_impl.
      exists k x. splits~. case_if~.
 Qed.
 
 (* internal use *)
 Lemma binds_impl_dom_impl : forall A `{Inhab B} (M:map A B) x v,
-  binds_impl M x v -> x \in dom_impl M.
-Proof using. introv IB K. unfolds binds_impl, dom_impl. set_norm. congruence. Qed.
+  binds_impl M x v -> 
+  x \in dom_impl M.
+Proof using. introv IB K. unfolds binds_impl, dom_impl. rew_set. congruence. Qed.
 
 (* LATER: avoid `{Inhab B}: if not empty, then inhab, else result true *)
 (* internal use *)
@@ -647,21 +623,21 @@ Lemma finite_to_finite_fold_support : forall A `{Inhab B} (M:map A B),
 Proof using.
   introv IB HM. lets (L&E): finite_inv_list_covers HM.
   applys finite_of_list_covers (LibList.map (fun x => (x, M[x])) L).
-  intros (k',x') Hk. set_norm. destruct Hk as (k&x&EQ&R). inverts EQ.
+  intros (k',x') Hk. rew_set. destruct Hk as (k&x&EQ&R). inverts EQ.
   forwards~: binds_impl_dom_impl R. forwards~ V: E k.
-  lets U: LibList.Mem_map (fun x => (x, M[x])) V. applys_eq U 2.
+  lets U: LibList.mem_map (fun x => (x, M[x])) V. applys_eq U 2.
   simpl. unfold read_impl. hnf in R. rewrite~ R.
 Qed.
 
 (* LATER: avoid `{Inhab B} *)
-Lemma fold_union : forall A `{Inhab B} C (m:monoid_def C) (f:A->B->C) (M N : map A B),
-  Monoid_comm m ->
+Lemma fold_union : forall A `{Inhab B} C (m:monoid_op C) (f:A->B->C) (M N : map A B),
+  Comm_monoid m ->
   finite M ->
-  finite N ->
+  finite N -> 
   M \# N ->
   fold m f (M \u N) = monoid_oper m (fold m f M) (fold m f N).
 Proof using.
-  introv IB Hm FM FN HD. do 3 rewrite fold_def_binds.
+  introv IB Hm FM FN HD. do 3 rewrite fold_eq_fold_pairs.
   match goal with |- context [ set_st ?X] =>
     cuts_rewrite (set_st X =
        \set{ p | exists k x, p = (k, x) /\ binds_impl M k x}
@@ -670,11 +646,11 @@ Proof using.
     apply~ finite_to_finite_fold_support.
     apply~ finite_to_finite_fold_support.
     rewrite disjoint_eq. (* TODO: applys disjoint_prove. *)
-    intros (k,x). set_norm. intros (k1&x1&E1&R1) (k2&x2&E2&R2).
+    intros (k,x). rew_set. intros (k1&x1&E1&R1) (k2&x2&E2&R2).
      inverts E1. forwards~: binds_impl_dom_impl R1.
      inverts E2. forwards~: binds_impl_dom_impl R2.
      applys* @disjoint_inv HD. typeclass.
-  set_norm. intros (k',x'). set_norm. iff (k&x&E&F) H.
+  rew_set. intros (k',x'). rew_set. iff (k&x&E&F) H.
     inverts E. simpl in F. unfolds union_impl, binds_impl. cases (N k).
       right. exists k x. inverts~ F.
       left. exists k x. auto.
@@ -682,7 +658,7 @@ Proof using.
       inverts E. exists k x. split~. forwards~: binds_impl_dom_impl R.
        cases (N k) as EN.
          false. applys~ @disjoint_inv k HD. typeclass.
-          unfold dom_impl. set_norm. congruence.
+          unfold dom_impl. rew_set. congruence.
          unfolds union_impl, binds_impl. rewrite~ EN.
       inverts E. exists k x. split~. forwards~: binds_impl_dom_impl R.
         unfolds union_impl, binds_impl. rewrite~ R.
@@ -691,13 +667,33 @@ Qed. (* todo: cleanup proof *)
 End Properties.
 
 
+(* -- LATER: equivalent definition of fold
+  Lemma fold_def_dom : forall A `{Inhab B} C (m:monoid_def C) (f:A->B->C) (M:map A B),
+    fold m f M = LibContainer.fold m (fun k => f k (M[k])) (dom M).
+    - E = dom M
+    - repr L E
+    - fold f (map i E) = fold (fun x => f (i x)) E
+    - i = fun x => (x, M[x])
+    - injective i -> repr E L -> repr (LibSet.map i E) (LibList.map i L)
+    - injective i -> No_duplicates L -> No_duplicates (map i L)
+    - repr E L -> repr E L' -> fold f E = fold f L'
+*)
+
 
 (* ---------------------------------------------------------------------- *)
 (** rewriting *)
 
-  (* TODO: this rewriting base might change *)
+(** EXPERIMENTAL -- beavior of [rew_map] might change
 
-Hint Rewrite @indom_update @update_read_neq @update_read_eq : rew_map.
+    The challenge is that it is not clear what we want to do facing
+    a read at index [i] on an update at index [j], when it is not obvious
+    from the context whether [i] and [j] might be equal. Often, it is
+    desirable to introduce a case analysis, but there are cases where
+    one would like to assume that if [i] and [j] are syntactically different,
+    i.e. one has not been already substituted for the other, then we wish
+    to issue a subgoal [i<>j]. *)
+
+Hint Rewrite @indom_update_eq @read_update_neq @read_update_same : rew_map.
 
 Tactic Notation "rew_map" :=
   autorewrite with rew_map.
@@ -706,7 +702,6 @@ Tactic Notation "rew_map" "in" hyp(H) :=
 Tactic Notation "rew_map" "in" "*" :=
   autorewrite_in_star_patch ltac:(fun tt => autorewrite with rew_map).
   (* autorewrite with rew_map in *. *)
-
 Tactic Notation "rew_map" "~" :=
   rew_map; auto_tilde.
 Tactic Notation "rew_map" "*" :=
@@ -759,44 +754,3 @@ End Instances.
 *)
 
 
-(* ---------------------------------------------------------------------- *)
-(* ---------------------------------------------------------------------- *)
-
-(* migration:
-
-  map_split ==> split_restrict_remove
-  map_split ==> split_restrict_remove_single
-  map_index_def ==> index_def
-  map_indom_update_already => LibMap.indom_update_already
-  map_indom_update_inv => LibMap.indom_update_inv
-  map_restrict_single ==> restrict_single
-  map_update_restrict ==> update_remove_one_eq
-  dom_restrict_in ==> index_remove_one_in
-  restrict_read ==> remove_one_read_neq
-  restrict_update ==> remove_one_update_neq
-
-  map_indom_update => indom_update
-  map_indom_update_self => indom_update_self
-  binds_inv => rewrite binds_def
-  binds_get => binds_read
-
-  map_update_read_eq => update_read_eq
-  map_update_read_neq => update_read_neq
-  map_update_read_if => update_read_if
-
-  dom_update_in => dom_update_index
-  dom_update_in_variant => dom_update_index'
-  dom_update_notin => dom_update
-  map_update_as_union => update_def_union
-  map_indom_update_already_inv => indom_update_already_inv
-
-  reduce_ => fold_
-
-*)
-
-
-(* LATER: is this deprecated?
-  Lemma binds_update_rem : forall A i j `{Inhab B} v w (M:map A B),
-    j \notindom' M -> binds (M[j:=w]) i v -> binds M i v.
-  Hint Resolve binds_update_rem.
-*)
